{
 "cells": [
  {
   "cell_type": "markdown",
   "metadata": {},
   "source": [
    "# Problem"
   ]
  },
  {
   "cell_type": "markdown",
   "metadata": {},
   "source": [
    "A wealthy investor provides a small amount of money $X_0$ for you to use to prove the effectiveness of your investment scheme over the next $N$ periods.  You are permitted to invest in the $N$-period binomial model, subject to the condition that the value of your portfolio is never allowed to be negative.  If at time $N$ the value of your portfolio $X_N$ is at least $\\gamma$, a positive constant specified the investor, then you will be given a large amount of money to manage for her.  Therefore, your problem is the following:\n",
    "\\begin{equation}\n",
    "\\text{Maximize} \\quad \\mathbb{P}(X_N\\geq \\gamma),\n",
    "\\end{equation}\n",
    "where $X_N$ is generated by a portfolio process beginning with the initial wealth $X_0$ and where the value $X_n$ of your portfolio process satisfies\n",
    "\\begin{equation}\n",
    "X_n\\geq 0, \\quad n=1,2,\\dots,N.\n",
    "\\end{equation}"
   ]
  },
  {
   "cell_type": "markdown",
   "metadata": {},
   "source": [
    "In the way that Problem 3.3.1 was reformulated as Problem 3.3.3, this problem may be reformulated as\n",
    "\\begin{equation}\n",
    "\\text{Maximize} \\quad \\mathbb{P}(X_N\\geq\\gamma)\n",
    "\\end{equation}\n",
    "subject to\n",
    "\\begin{align}\n",
    "&\\tilde{\\mathbb{E}}\\frac{X_N}{(1+r)^N}=X_0,\\\\\n",
    "&X_n\\geq 0, \\quad n=1,2,\\dots,N.\n",
    "\\end{align}"
   ]
  },
  {
   "cell_type": "markdown",
   "metadata": {},
   "source": [
    "(i) Show that if $X_N\\geq 0$, then $X_n\\geq 0$ for all $n$."
   ]
  },
  {
   "cell_type": "markdown",
   "metadata": {},
   "source": [
    "(ii) Consider the function\n",
    "\\begin{align}\n",
    "U(x)&=0, \\quad \\text{ if } 0\\leq x<\\gamma,\\\\\n",
    "&=1, \\quad \\text{ if } x\\geq\\gamma.\n",
    "\\end{align}\n",
    "Show that for each fixed $y>0$, we have\n",
    "\\begin{equation}\n",
    "U(x)-yx\\leq U(I(y))-yI(y) \\quad\\forall x\\geq 0,\n",
    "\\end{equation}\n",
    "where\n",
    "\\begin{align}\n",
    "I(y)&=\\gamma, \\quad \\text{ if } 0<y\\leq\\frac{1}{y},\\\\\n",
    "&=0, \\quad \\text{ if } y>\\frac{1}{y}.\n",
    "\\end{align}"
   ]
  },
  {
   "cell_type": "markdown",
   "metadata": {},
   "source": [
    "(iii) Assume there is a solution $\\lambda$ to the equation\n",
    "\\begin{equation}\n",
    "\\mathbb{E}\\left[\\frac{Z}{(1+r)^N}I\\left(\\frac{\\lambda Z}{(1+r)^N}\\right)\\right]=X_0.\n",
    "\\end{equation}\n",
    "following the argument of Exercise 3.8, show that the optimal $X_N$ is given by\n",
    "\\begin{equation}\n",
    "X_N^*=I\\left(\\frac{\\lambda Z}{(1+r)^N}\\right).\n",
    "\\end{equation}"
   ]
  },
  {
   "cell_type": "markdown",
   "metadata": {},
   "source": [
    "(iv) As we did to obtain Problem 3.3.5, let us list the $M=2^N$ possible coin toss sequences, labeling them $\\omega^1,\\dots,\\omega^M$, and then define $\\zeta_m=\\zeta(\\omega^m)$, $p_m=\\mathbb{P}(\\omega^m)$.  However, here we list these sequences in ascending order of $\\zeta_m$, i.e., we label the coin toss sequences so that\n",
    "\\begin{equation}\n",
    "\\zeta_1\\leq\\zeta_2\\leq\\dots\\leq\\zeta_M.\n",
    "\\end{equation}\n",
    "Show that the assumption that there is a solution $\\lambda$ to (3.6.4) is equivalent to assuming that for some positive integer $K$ we have $\\zeta_K<\\zeta_{K+1}$ and\n",
    "\\begin{equation}\n",
    "\\sum_{m=1}^{K}\\zeta_mp_m=\\frac{X_0}{\\gamma}.\n",
    "\\end{equation}"
   ]
  },
  {
   "cell_type": "markdown",
   "metadata": {},
   "source": [
    "(v) Show that $X_N^*$ is given by\n",
    "\\begin{align}\n",
    "X_N(\\omega^m)&=\\gamma, \\quad \\text{ if } m\\leq K,\\\\\n",
    "&=0, \\quad \\text{ if } m\\geq K+1.\n",
    "\\end{align}"
   ]
  },
  {
   "cell_type": "markdown",
   "metadata": {},
   "source": [
    "# Answer"
   ]
  },
  {
   "cell_type": "markdown",
   "metadata": {},
   "source": [
    "(i) Recall the risk-neutral pricing formula for the portfolio wealth process\n",
    "\\begin{equation}\n",
    "X_n=\\tilde{\\mathbb{E}}\\left[\\frac{X_N}{(1+r)^{N-n}}\\right].\n",
    "\\end{equation}\n",
    "If $X_N\\geq 0$, then the expectation on the right is greater than or equal to $0$, and hence $X_n\\geq 0$ as well. $\\square$"
   ]
  },
  {
   "cell_type": "markdown",
   "metadata": {},
   "source": [
    "(ii) Our approach is to find an upper bound for the expression $U(x)-yx$, and at the same time a lower bound for $U(I(y))-yI(y)$. There are four cases, which we list below\n",
    "\\begin{align}\n",
    "0\\leq &x<\\gamma \\quad \\text{ and } &0<y\\leq\\frac{1}{\\gamma},\\\\\n",
    "0\\leq &x<\\gamma \\quad \\text{ and } &y>\\frac{1}{\\gamma},\\\\\n",
    "&x\\geq\\gamma \\quad \\text{ and } &0<y\\leq\\frac{1}{\\gamma},\\\\\n",
    "&x\\geq\\gamma \\quad \\text{ and } &y>\\frac{1}{\\gamma}.\n",
    "\\end{align}"
   ]
  },
  {
   "cell_type": "markdown",
   "metadata": {},
   "source": [
    "For the first case, we have\n",
    "\\begin{equation}\n",
    "U(x)-yx=0-yx\\leq 0,\n",
    "\\end{equation}\n",
    "and\n",
    "\\begin{equation}\n",
    "U(I(y))-yI(y)=U(\\gamma)-y\\gamma=1-y\\gamma\\geq 1-\\frac{1}{\\gamma}\\gamma=0\\geq U(x).\n",
    "\\end{equation}"
   ]
  },
  {
   "cell_type": "markdown",
   "metadata": {},
   "source": [
    "For the second case, we have\n",
    "\\begin{equation}\n",
    "U(x)-yx=0-yx\\leq 0,\n",
    "\\end{equation}\n",
    "and\n",
    "\\begin{equation}\n",
    "U(I(y))-yI(y)=U(0)-y\\times 0=0-y\\times 0=0\\geq U(x).\n",
    "\\end{equation}"
   ]
  },
  {
   "cell_type": "markdown",
   "metadata": {},
   "source": [
    "For the third case, we have\n",
    "\\begin{equation}\n",
    "U(x)-yx=1-yx\\leq 1-y\\gamma,\n",
    "\\end{equation}\n",
    "and\n",
    "\\begin{equation}\n",
    "U(I(y))-I(y)=U(\\gamma)-y\\gamma=1-y\\gamma\\geq U(x).\n",
    "\\end{equation}"
   ]
  },
  {
   "cell_type": "markdown",
   "metadata": {},
   "source": [
    "For the fourth case, we have\n",
    "\\begin{equation}\n",
    "U(x)-yx=1-yx\\leq 1-\\frac{1}{\\gamma}\\gamma=1-1=0,\n",
    "\\end{equation}\n",
    "\\begin{equation}\n",
    "U(I(y))-yI(y)=U(0)-y\\times 0=0-y\\times 0=0\\geq U(x). \\square\n",
    "\\end{equation}"
   ]
  },
  {
   "cell_type": "markdown",
   "metadata": {},
   "source": [
    "(iii) In the part (ii) of this exercise, we showed that the function of $x$ given by $U(x)-yx$ is maximized by $x=I(y)$.  In other words,\n",
    "\\begin{equation}\n",
    "U(x)-yx\\leq U(I(y))-yI(y).\n",
    "\\end{equation}\n",
    "Combined with the assumption that there exists a $\\lambda$ such that\n",
    "\\begin{equation}\n",
    "\\mathbb{E}\\left[\\frac{Z}{(1+r)^N}I\\left(\\frac{\\lambda Z}{(1+r)^N}\\right)\\right]=X_0,\n",
    "\\end{equation}\n",
    "we have satisfied the hypotheses of Exercise 3.8.  Hence, the result of Exercise 3.8 (ii) immediately gives us that\n",
    "\\begin{equation}\n",
    "X^*_N=I\\left(\\frac{\\lambda Z}{(1+r)^N}\\right).\\square\n",
    "\\end{equation}"
   ]
  },
  {
   "cell_type": "markdown",
   "metadata": {},
   "source": [
    "(iv) $\\Rightarrow)$ Assume\n",
    "\\begin{equation}\n",
    "\\mathbb{E}\\left[\\frac{Z}{(1+r)^N}I\\left(\\frac{\\lambda Z}{(1+r)^N}\\right)\\right]=X_0,\n",
    "\\end{equation}\n",
    "or, equivalently,\n",
    "\\begin{equation}\n",
    "\\mathbb{E}\\left[\\zeta I\\left(\\lambda\\zeta\\right)\\right]=X_0.\n",
    "\\end{equation}\n",
    "Expanding the left hand side, we obtain\n",
    "\\begin{equation}\n",
    "\\sum_{m=1}^{M}p_m\\zeta_mI(\\lambda\\zeta_m)=\n",
    "\\sum_{\\substack{m\\\\\\lambda\\zeta_m>\\frac{1}{\\gamma}}}p_m\\zeta_mI(\\lambda\\zeta_m)+\\sum_{\\substack{m\\\\0<\\lambda\\zeta_m\\leq\\frac{1}{\\gamma}}}p_m\\zeta_mI(\\lambda\\zeta_m).\n",
    "\\end{equation}"
   ]
  },
  {
   "cell_type": "markdown",
   "metadata": {},
   "source": [
    "Because $I(y)=0$ whenever $y>\\frac{1}{\\gamma}$, the left term above drops out and we are left with\n",
    "\\begin{equation}\n",
    "\\sum_{\\substack{m\\\\0<\\lambda\\zeta_m\\leq\\frac{1}{\\gamma}}}p_m\\zeta_m\\gamma.\n",
    "\\end{equation}\n",
    "Note that the set of values of $0<\\lambda\\zeta_m\\leq\\frac{1}{\\gamma}$ cannot be empty, otherwise $X_0=0$, and this violates our hypothesis that $X_0>0$.\n",
    "Next, we divde both sides by $\\lambda$ and obtain\n",
    "\\begin{equation}\n",
    "\\sum_{\\substack{m\\\\0<\\lambda\\zeta_m\\leq\\frac{1}{\\gamma}}}p_m\\zeta_m=\\frac{X_0}{\\gamma}.\n",
    "\\end{equation}"
   ]
  },
  {
   "cell_type": "markdown",
   "metadata": {},
   "source": [
    "Now note that we cannot have $m$ run though all the indices (i.e. $m=1,\\dots,M$), because then left-hand side of the expression would equal $\\mathbb{E}\\left[\\zeta\\right]=1$, and we'd have $1=\\frac{X_0}{\\gamma}$.  But $X_0$ and $\\gamma$ are allowed to vary freely, and that condition would violate that.  Additionally, note that the problem is trivial if $X_0=\\gamma$, because in that case the investor can guarantee that he hits the goal (of having wealth greater than or equal to $\\gamma$ at time $N$) by investing in the money market at every time period.  In short, the problem is only non-trivial if $X_0<\\gamma$, and this implies that $m$ cannot run through all the indices."
   ]
  },
  {
   "cell_type": "markdown",
   "metadata": {},
   "source": [
    "Now note that if $m$ cannot run through all the indices, then this is equivalent to saying that there is a positive integer $K$ such that\n",
    "\\begin{equation}\n",
    "\\sum_{m=1}^K\\zeta_mp_m=\\frac{X_0}{\\gamma}.\n",
    "\\end{equation}\n",
    "It only remains to show that $\\zeta_K<\\zeta_{K+1}$.  But this is guaranteed by the fact that, according to the way we split the summation, we would have $\\lambda\\zeta_{K+1}>\\frac{1}{\\gamma}$, and $0\\leq\\lambda\\zeta_{K+1}\\leq\\frac{1}{\\gamma}$, and this implies $\\zeta_K<\\zeta_{K+1}$."
   ]
  },
  {
   "cell_type": "markdown",
   "metadata": {},
   "source": [
    "$\\Leftarrow)$ Now assume that for some positive integer $K$ we have $\\zeta_{K}<\\zeta_{K+1}$ and\n",
    "\\begin{equation}\n",
    "\\sum_{m=1}^{K}\\zeta_mp_m=\\frac{X_0}{\\gamma}.\n",
    "\\end{equation}\n",
    "This implies that\n",
    "\\begin{equation}\n",
    "\\sum_{m=1}^{K}\\zeta_mp_m\\gamma=X_0.\n",
    "\\end{equation}\n",
    "Note that the above expression is equivalent to\n",
    "\\begin{equation}\n",
    "\\sum_{m=1}^{K}\\zeta_mp_mI(\\lambda\\zeta_m)+\\sum_{m=K+1}^{M}\\zeta_mp_mI(\\lambda\\zeta_m)=X_0,\n",
    "\\end{equation}\n",
    "if we can find a $\\lambda$ such that\n",
    "\\begin{align}\n",
    "&I(\\lambda\\zeta_m)=\\gamma \\quad \\text{for } 1\\leq m\\leq K,\\\\\n",
    "&I(\\lambda\\zeta_m)=0 \\quad \\text{for } K+1\\leq m\\leq M,\n",
    "\\end{align}\n",
    "which is equivalent, by definition of $I(y)$, to requiring that\n",
    "\\begin{align}\n",
    "0<&\\lambda\\zeta_m\\leq\\frac{1}{\\gamma} \\quad \\text{for } 1\\leq m\\leq K,\\\\\n",
    "&\\lambda\\zeta_m>\\frac{1}{\\gamma} \\quad \\text{for } K+1\\leq m\\leq M.\n",
    "\\end{align}"
   ]
  },
  {
   "cell_type": "markdown",
   "metadata": {},
   "source": [
    "Because the $\\zeta_m$ are indexed in ascending order, we can satisfy the two equations above if we can find a $\\lambda>0$ such that\n",
    "\\begin{gather}\n",
    "\\lambda\\zeta_K\\leq\\frac{1}{\\gamma}\\Rightarrow\\lambda\\leq\\frac{1}{\\gamma\\zeta_K},\\\\\n",
    "\\lambda\\zeta_{K+1}>\\frac{1}{\\gamma}\\Rightarrow\\lambda>\\frac{1}{\\gamma\\zeta_{K+1}}.\n",
    "\\end{gather}\n",
    "We can indeed find such a $\\lambda$ because $\\zeta_K<\\zeta_{K+1}$."
   ]
  },
  {
   "cell_type": "markdown",
   "metadata": {},
   "source": [
    "In short, for appropriate $\\lambda$, the expression\n",
    "\\begin{equation}\n",
    "\\sum_{m=1}^{K}\\zeta_mp_mI(\\lambda\\zeta_m)+\\sum_{m=K+1}^{M}\\zeta_mp_mI(\\lambda\\zeta_m)=X_0\n",
    "\\end{equation}\n",
    "is justified.  Now it is just a matter of rewriting the left hand of the expression, and obtained the desired result:\n",
    "\\begin{align}\n",
    "\\sum_{m=1}^{K}\\zeta_mp_mI(\\lambda\\zeta_m)&+\\sum_{m=K+1}^{M}\\zeta_mp_mI(\\lambda\\zeta_m)=\\sum_{m=1}^{M}\\zeta_mp_mI(\\lambda\\zeta_m)\\\\\n",
    "&=\\mathbb{E}\\left[\\zeta I\\left(\\lambda\\zeta\\right)\\right]\\\\\n",
    "&=\\mathbb{E}\\left[\\frac{Z}{(1+r)^N}I\\left(\\frac{\\lambda Z}{(1+r)^N}\\right)\\right]=X_0.\\square\n",
    "\\end{align}"
   ]
  },
  {
   "cell_type": "markdown",
   "metadata": {},
   "source": [
    "(v) Assume there is a $\\lambda$ satisfying\n",
    "\\begin{equation}\n",
    "\\mathbb{E}\\left[\\frac{Z}{(1+r)^N}I\\left(\\frac{\\lambda Z}{(1+r)^N}\\right)\\right]=X_0.\n",
    "\\end{equation}\n",
    "Now let \n",
    "\\begin{equation}\n",
    "X^*_N=I\\left(\\lambda\\frac{Z}{(1+r)^N}\\right)=I\\left(\\lambda\\zeta\\right).\n",
    "\\end{equation}\n",
    "In part (iv) of this exercise, we showed that that $\\lambda$ might be, it has to satisfy the conditions\n",
    "\\begin{align}\n",
    "&I(\\lambda\\zeta_m)=I(\\lambda\\zeta(\\omega^m))=\\gamma \\quad \\text{for } 1\\leq m\\leq K,\\\\\n",
    "&I(\\lambda\\zeta_m)=I(\\lambda\\zeta(\\omega^m))=0 \\quad \\text{for } K+1\\leq m\\leq M.\n",
    "\\end{align}\n",
    "Hence\n",
    "\\begin{align}\n",
    "&X^*_N(\\omega^m)=I(\\lambda\\zeta_m)=I(\\lambda\\zeta(\\omega^m))=\\gamma \\quad \\text{for } 1\\leq m\\leq K,\\\\\n",
    "&X^*_N(\\omega^m)=I(\\lambda\\zeta_m)=I(\\lambda\\zeta(\\omega^m))=0 \\quad \\text{for } K+1\\leq m\\leq M. \\square\n",
    "\\end{align}"
   ]
  }
 ],
 "metadata": {
  "kernelspec": {
   "display_name": "Python 3",
   "language": "python",
   "name": "python3"
  },
  "language_info": {
   "codemirror_mode": {
    "name": "ipython",
    "version": 3
   },
   "file_extension": ".py",
   "mimetype": "text/x-python",
   "name": "python",
   "nbconvert_exporter": "python",
   "pygments_lexer": "ipython3",
   "version": "3.7.6"
  }
 },
 "nbformat": 4,
 "nbformat_minor": 4
}
